SeqLast.dfy
@@ -1,0 +1,23 @@
+module SeqLast {
+
+  // returns the last element in the sequence
+  function method last<E>(s: seq<E>): E
+    requires |s| > 0;
+  {
+    s[|s|-1]
+  }
+
+  // returns the sequence slice up to but not including the last element
+  function method drop_last<E>(s: seq<E>): seq<E> 
+  requires |s| > 0;
+  {
+    s[..|s|-1]
+  }
+
+  // concatenating everything but the last element + the last element results in the original seq 
+  lemma lemma_last<T>(s: seq<T>)
+    requires |s| > 0;
+    ensures  drop_last(s) + [last(s)] == s;
+  {
+  }
+}
