SeqOfSeq.dfy
@@ -1,0 +1,22 @@
+include "SeqLast.dfy"
+
+module SeqOfSeq {
+
+  import opened SeqLast
+
+  /*concatenates a sequence of sequences into a single sequence. 
+  Works by adding elements in order from first to last */
+  function method seq_concat<T>(seqs: seq<seq<T>>): seq<T>
+  decreases |seqs|
+  {
+    if |seqs| == 0 then []
+    else seqs[0] + seq_concat(seqs[1..])
+  }
+
+  // turns a sequence of sequences into a single sequence and returns the result
+  function method {:opaque} concat_seq<A>(a: seq<seq<A>>): seq<A>
+  {
+    if |a| == 0 then [] else concat_seq(drop_last(a)) + last(a)
+  }
+
+}
